restore ArrayGroup definitions

src/cddl/spec/CDDL.Spec.ArrayGroup.fsti
@@ -85,7 +85,7 @@ let rec opt_precedes_opt_precedes_list
   | a :: q -> opt_precedes_opt_precedes_list q b
 
 [@@ noextract_to "krml"]
-let array_group3 (bound: option Cbor.cbor) = (l: list Cbor.cbor { opt_precedes_list l bound }) -> Pure (option (list Cbor.cbor & list Cbor.cbor))
+let array_group (bound: option Cbor.cbor) = (l: list Cbor.cbor { opt_precedes_list l bound }) -> Pure (option (list Cbor.cbor & list Cbor.cbor))
   (requires True)
   (ensures (fun l' -> match l' with
   | None -> True
@@ -93,13 +93,13 @@ let array_group3 (bound: option Cbor.cbor) = (l: list Cbor.cbor { opt_precedes_l
   ))
 
 noextract
-let array_group3_equiv
+let array_group_equiv
   #b
-  (g1 g2: array_group3 b)
+  (g1 g2: array_group b)
 : Tot prop
 = forall l . g1 l == g2 l
 
-let array_group3_always_false #b : array_group3 b = fun _ -> None
+let array_group_always_false #b : array_group b = fun _ -> None
 
 let rec opt_precedes_list_assoc
   (#t1 #t2: Type)
@@ -112,8 +112,8 @@ let rec opt_precedes_list_assoc
   | [] -> ()
   | _ :: q1 -> opt_precedes_list_assoc q1 l2 b
 
-let array_group3_empty #b : array_group3 b = fun x -> Some ([], x)
-let array_group3_concat #b (a1 a3: array_group3 b) : array_group3 b =
+let array_group_empty #b : array_group b = fun x -> Some ([], x)
+let array_group_concat #b (a1 a3: array_group b) : array_group b =
   (fun l ->
     match a1 l with
     | None -> None
@@ -123,30 +123,30 @@ let array_group3_concat #b (a1 a3: array_group3 b) : array_group3 b =
     end
   )
 
-let array_group3_concat_equiv
+let array_group_concat_equiv
   #b
-  (a1 a1' a2 a2' : array_group3 b)
+  (a1 a1' a2 a2' : array_group b)
 : Lemma
-  (requires ((a1 `array_group3_equiv` a1') /\ (a2 `array_group3_equiv` a2')))
-  (ensures ((a1 `array_group3_concat` a2) `array_group3_equiv` (a1' `array_group3_concat` a2')))
+  (requires ((a1 `array_group_equiv` a1') /\ (a2 `array_group_equiv` a2')))
+  (ensures ((a1 `array_group_concat` a2) `array_group_equiv` (a1' `array_group_concat` a2')))
 = ()
 
-val array_group3_concat_assoc
+val array_group_concat_assoc
   (#b: _)
-  (a1 a2 a3: array_group3 b)
+  (a1 a2 a3: array_group b)
 : Lemma
-  (array_group3_concat a1 (array_group3_concat a2 a3) `array_group3_equiv`
-    array_group3_concat (array_group3_concat a1 a2) a3)
+  (array_group_concat a1 (array_group_concat a2 a3) `array_group_equiv`
+    array_group_concat (array_group_concat a1 a2) a3)
   [SMTPatOr [
-//    [SMTPat (array_group3_concat a1 (array_group3_concat a2 a3))];
-    [SMTPat (array_group3_concat (array_group3_concat a1 a2) a3)]
+//    [SMTPat (array_group_concat a1 (array_group_concat a2 a3))];
+    [SMTPat (array_group_concat (array_group_concat a1 a2) a3)]
   ]]
 
-let array_group3_concat_unique_strong
-  #b (a1 a3: array_group3 b)
+let array_group_concat_unique_strong
+  #b (a1 a3: array_group b)
 : Tot prop
 = (forall (l: (l: list Cbor.cbor { opt_precedes_list l b })) (l' rem: list Cbor.cbor) .
-    array_group3_concat a1 a3 l == Some (l', rem) <==> (
+    array_group_concat a1 a3 l == Some (l', rem) <==> (
       (exists (l1 l2 l3: list Cbor.cbor) .
         l == l1 `List.Tot.append` l2 /\
         a1 l1 == Some (l1, []) /\
@@ -158,55 +158,55 @@ let array_group3_concat_unique_strong
     a1 (l1 `List.Tot.append` l2) == Some (l1, l2)
   )
 
-let array_group3_concat_unique_strong_equiv
-  #b (a1 a1' a3 a3': array_group3 b)
+let array_group_concat_unique_strong_equiv
+  #b (a1 a1' a3 a3': array_group b)
 : Lemma
   (requires (
-    array_group3_equiv a1 a1' /\
-    array_group3_equiv a3 a3'
+    array_group_equiv a1 a1' /\
+    array_group_equiv a3 a3'
   ))
   (ensures (
-    array_group3_concat_unique_strong a1 a3 <==>
-    array_group3_concat_unique_strong a1' a3'
+    array_group_concat_unique_strong a1 a3 <==>
+    array_group_concat_unique_strong a1' a3'
   ))
-= array_group3_concat_equiv a1 a1' a3 a3'
+= array_group_concat_equiv a1 a1' a3 a3'
 
-let array_group3_strong_prefix
-  #b (a1: array_group3 b)
+let array_group_strong_prefix
+  #b (a1: array_group b)
 : Tot prop
 = forall (l1 l2: (l: list Cbor.cbor { opt_precedes_list l b })) .
     (a1 l1 == Some (l1, []) <==> a1 (l1 `List.Tot.append` l2) == Some (l1, l2))
 
-val array_group3_concat_unique_strong_strong_prefix
-  (#b: _) (a1 a2: array_group3 b)
+val array_group_concat_unique_strong_strong_prefix
+  (#b: _) (a1 a2: array_group b)
 : Lemma
   (requires (
-    array_group3_concat_unique_strong a1 a2 /\
-    array_group3_strong_prefix a2
+    array_group_concat_unique_strong a1 a2 /\
+    array_group_strong_prefix a2
   ))
   (ensures (
-    array_group3_strong_prefix (array_group3_concat a1 a2)
+    array_group_strong_prefix (array_group_concat a1 a2)
   ))
 
-let array_group3_choice #b (a1 a3: array_group3 b) : array_group3 b =
+let array_group_choice #b (a1 a3: array_group b) : array_group b =
   fun l -> match a1 l with
     | None -> a3 l
     | Some l3 -> Some l3
 
-let array_group3_disjoint #b (a1 a2: array_group3 b) : Tot prop
+let array_group_disjoint #b (a1 a2: array_group b) : Tot prop
 = (forall (l: list Cbor.cbor { opt_precedes_list l b }) . ~ (Some? (a1 l) /\ Some? (a2 l)))
 
-val array_group3_concat_unique_strong_choice_left #b (a1 a2 a3: array_group3 b) : Lemma
+val array_group_concat_unique_strong_choice_left #b (a1 a2 a3: array_group b) : Lemma
   (requires (
-    array_group3_concat_unique_strong a1 a3 /\
-    array_group3_concat_unique_strong a2 a3 /\
-    array_group3_disjoint a1 a2
+    array_group_concat_unique_strong a1 a3 /\
+    array_group_concat_unique_strong a2 a3 /\
+    array_group_disjoint a1 a2
   ))
   (ensures (
-    array_group3_concat_unique_strong (array_group3_choice a1 a2) a3
+    array_group_concat_unique_strong (array_group_choice a1 a2) a3
   ))
 
-let rec array_group3_zero_or_more' #b (a: array_group3 b) (l: list Cbor.cbor { opt_precedes_list l b }) : Pure (option (list Cbor.cbor & list Cbor.cbor))
+let rec array_group_zero_or_more' #b (a: array_group b) (l: list Cbor.cbor { opt_precedes_list l b }) : Pure (option (list Cbor.cbor & list Cbor.cbor))
   (requires True)
   (ensures (fun l' -> match l' with None -> True | Some (l1, l2) -> l == l1 `List.Tot.append` l2))
   (decreases (List.Tot.length l))
@@ -218,45 +218,45 @@ let rec array_group3_zero_or_more' #b (a: array_group3 b) (l: list Cbor.cbor { o
     if Nil? l1
     then Some (l1, l2)
     else
-      begin match array_group3_zero_or_more' a l2 with
+      begin match array_group_zero_or_more' a l2 with
       | None -> None
       | Some (l2', l3) -> List.Tot.append_assoc l1 l2' l3; Some (List.Tot.append l1 l2', l3)
       end
 
-let array_group3_zero_or_more #b : array_group3 b -> array_group3 b = array_group3_zero_or_more'
+let array_group_zero_or_more #b : array_group b -> array_group b = array_group_zero_or_more'
 
-val array_group3_zero_or_more_some
+val array_group_zero_or_more_some
   (#b: _)
-  (a: array_group3 b)
+  (a: array_group b)
   (l: list Cbor.cbor { opt_precedes_list l b })
 : Lemma
-  (ensures (Some? (array_group3_zero_or_more a l)))
-  [SMTPat (array_group3_zero_or_more a l)]
+  (ensures (Some? (array_group_zero_or_more a l)))
+  [SMTPat (array_group_zero_or_more a l)]
 
-val array_group3_zero_or_more_equiv (#b: _)
- (a1 a2: array_group3 b)
+val array_group_zero_or_more_equiv (#b: _)
+ (a1 a2: array_group b)
 : Lemma
-  (requires array_group3_equiv a1 a2)
-  (ensures array_group3_equiv (array_group3_zero_or_more a1) (array_group3_zero_or_more a2))
-  [SMTPat (array_group3_equiv (array_group3_zero_or_more a1) (array_group3_zero_or_more a2))]
+  (requires array_group_equiv a1 a2)
+  (ensures array_group_equiv (array_group_zero_or_more a1) (array_group_zero_or_more a2))
+  [SMTPat (array_group_equiv (array_group_zero_or_more a1) (array_group_zero_or_more a2))]
 
-val array_group3_concat_unique_strong_zero_or_more_left
-  (#b: _) (a1 a2: array_group3 b)
+val array_group_concat_unique_strong_zero_or_more_left
+  (#b: _) (a1 a2: array_group b)
 : Lemma
   (requires (
-    array_group3_disjoint a1 a2 /\
-    array_group3_concat_unique_strong a1 a1 /\
-    array_group3_concat_unique_strong a1 a2
+    array_group_disjoint a1 a2 /\
+    array_group_concat_unique_strong a1 a1 /\
+    array_group_concat_unique_strong a1 a2
   ))
   (ensures (
-    array_group3_concat_unique_strong (array_group3_zero_or_more a1) a2
+    array_group_concat_unique_strong (array_group_zero_or_more a1) a2
   ))
 
-let array_group3_concat_unique_weak
-  #b (a1 a3: array_group3 b)
+let array_group_concat_unique_weak
+  #b (a1 a3: array_group b)
 : Tot prop
 = (forall (l: (l: list Cbor.cbor { opt_precedes_list l b })) .
-    array_group3_concat a1 a3 l == Some (l, []) ==> (
+    array_group_concat a1 a3 l == Some (l, []) ==> (
       (exists (l1 l2: list Cbor.cbor) .
         a1 l == Some (l1, l2) /\
         a1 l1 == Some (l1, []) /\
@@ -267,31 +267,47 @@ let array_group3_concat_unique_weak
     a1 (l1 `List.Tot.append` l2) == Some (l1, l2)
   )
 
-let array_group3_concat_unique_weak_elim2
-  #b (a1 a3: array_group3 b)
+let array_group_concat_unique_weak_elim1
+  #b (a1 a3: array_group b)
+  (l: list Cbor.cbor { opt_precedes_list l b })
+: Lemma
+  (requires (
+    array_group_concat_unique_weak a1 a3 /\
+    array_group_concat a1 a3 l == Some (l, [])
+  ))
+  (ensures (
+      exists (l1 l2: list Cbor.cbor) .
+        a1 l == Some (l1, l2) /\
+        a1 l1 == Some (l1, []) /\
+        a3 l2 == Some (l2, [])
+  ))
+= ()
+
+let array_group_concat_unique_weak_elim2
+  #b (a1 a3: array_group b)
   (l1 l2: (l: list Cbor.cbor { opt_precedes_list l b }))
 : Lemma
   (requires (
-    array_group3_concat_unique_weak a1 a3 /\
+    array_group_concat_unique_weak a1 a3 /\
     a1 l1 == Some (l1, []) /\
     a3 l2 == Some (l2, [])
   ))
   (ensures a1 (l1 `List.Tot.append` l2) == Some (l1, l2))
 = ()
 
-val array_group3_concat_unique_weak_intro
-  (#b: _) (a1 a3: array_group3 b)
+val array_group_concat_unique_weak_intro
+  (#b: _) (a1 a3: array_group b)
   (prf1:
     (l: (l: list Cbor.cbor { opt_precedes_list l b })) ->
     Lemma
-    (requires array_group3_concat a1 a3 l == Some (l, []))
+    (requires array_group_concat a1 a3 l == Some (l, []))
     (ensures
       (exists (l1 l2: list Cbor.cbor) .
         a1 l == Some (l1, l2) /\
         a1 l1 == Some (l1, []) /\
         a3 l2 == Some (l2, [])
     ))
-//    [SMTPat (array_group3_concat a1 a3 l)]
+//    [SMTPat (array_group_concat a1 a3 l)]
   )
   (prf2:
     (l1: (l: list Cbor.cbor { opt_precedes_list l b })) ->
@@ -306,7 +322,7 @@ val array_group3_concat_unique_weak_intro
 //    [SMTPat (a1 (l1 `List.Tot.append` l2))]
   )
 : Lemma
-  (array_group3_concat_unique_weak a1 a3)
+  (array_group_concat_unique_weak a1 a3)
 
 let list_append_l_nil
   (#t: Type)
@@ -316,190 +332,190 @@ let list_append_l_nil
   [SMTPat (l `List.Tot.append` [])]
 = List.Tot.append_l_nil l
 
-val array_group3_concat_unique_weak_zero_or_more_left
-  (#b: _) (a1 a2: array_group3 b)
+val array_group_concat_unique_weak_zero_or_more_left
+  (#b: _) (a1 a2: array_group b)
 : Lemma
   (requires (
-    array_group3_disjoint a1 a2 /\
-    array_group3_concat_unique_strong a1 a1 /\
-    array_group3_concat_unique_weak a1 a2
+    array_group_disjoint a1 a2 /\
+    array_group_concat_unique_strong a1 a1 /\
+    array_group_concat_unique_weak a1 a2
   ))
   (ensures (
-    array_group3_concat_unique_weak (array_group3_zero_or_more a1) a2
+    array_group_concat_unique_weak (array_group_zero_or_more a1) a2
   ))
 
-val array_group3_concat_unique_weak_zero_or_more_right
-  (#b: _) (a1 a2: array_group3 b)
+val array_group_concat_unique_weak_zero_or_more_right
+  (#b: _) (a1 a2: array_group b)
 : Lemma
   (requires (
-    array_group3_concat_unique_strong a1 a2
+    array_group_concat_unique_strong a1 a2
   ))
   (ensures (
-    array_group3_concat_unique_weak a1 (array_group3_zero_or_more a2)
+    array_group_concat_unique_weak a1 (array_group_zero_or_more a2)
   ))
 
-val array_group3_concat_unique_weak_zero_or_more
-  (#b: _) (a1 a2: array_group3 b)
+val array_group_concat_unique_weak_zero_or_more
+  (#b: _) (a1 a2: array_group b)
 : Lemma
   (requires (
-    array_group3_concat_unique_strong a1 a1 /\
-    array_group3_concat_unique_strong a1 a2 /\
-    array_group3_disjoint a1 a2
+    array_group_concat_unique_strong a1 a1 /\
+    array_group_concat_unique_strong a1 a2 /\
+    array_group_disjoint a1 a2
   ))
   (ensures (
-    array_group3_concat_unique_weak (array_group3_zero_or_more a1) (array_group3_zero_or_more a2)
+    array_group_concat_unique_weak (array_group_zero_or_more a1) (array_group_zero_or_more a2)
   ))
 
-val array_group3_concat_unique_weak_choice_right #b (a1 a2 a3: array_group3 b) : Lemma
+val array_group_concat_unique_weak_choice_right #b (a1 a2 a3: array_group b) : Lemma
   (requires (
-    array_group3_concat_unique_weak a1 a2 /\
-    array_group3_concat_unique_weak a1 a3
+    array_group_concat_unique_weak a1 a2 /\
+    array_group_concat_unique_weak a1 a3
   ))
   (ensures (
-    array_group3_concat_unique_weak a1 (array_group3_choice a2 a3)
+    array_group_concat_unique_weak a1 (array_group_choice a2 a3)
   ))
 
-val array_group3_concat_unique_weak_choice_left #b (a1 a2 a3: array_group3 b) : Lemma
+val array_group_concat_unique_weak_choice_left #b (a1 a2 a3: array_group b) : Lemma
   (requires (
-    array_group3_concat_unique_weak a1 a3 /\
-    array_group3_concat_unique_weak a2 a3 /\
-    array_group3_disjoint a1 a2
+    array_group_concat_unique_weak a1 a3 /\
+    array_group_concat_unique_weak a2 a3 /\
+    array_group_disjoint a1 a2
   ))
   (ensures (
-    array_group3_concat_unique_weak (array_group3_choice a1 a2) a3
+    array_group_concat_unique_weak (array_group_choice a1 a2) a3
   ))
 
 #restart-solver
 let array_group_concat_unique_weak_concat_left
-  (g1 g2 g3: array_group3 None)
+  (g1 g2 g3: array_group None)
 : Lemma
   (requires
-    array_group3_concat_unique_weak g1 g2 /\
-    array_group3_concat_unique_weak g2 g3 /\    
-    array_group3_concat_unique_weak g1 (g2 `array_group3_concat` g3)
+    array_group_concat_unique_weak g1 g2 /\
+    array_group_concat_unique_weak g2 g3 /\    
+    array_group_concat_unique_weak g1 (g2 `array_group_concat` g3)
   )
   (ensures
-    array_group3_concat_unique_weak (g1 `array_group3_concat` g2) g3
+    array_group_concat_unique_weak (g1 `array_group_concat` g2) g3
   )
-=   let a1 = g1 `array_group3_concat` g2 in
+=   let a1 = g1 `array_group_concat` g2 in
     let a3 = g3 in
-    array_group3_concat_unique_weak_intro a1 a3
+    array_group_concat_unique_weak_intro a1 a3
       (fun l -> ())
       (fun l1 l2 ->
         let Some (l1l, l1r) = g1 l1 in
         List.Tot.append_assoc l1l l1r l2
       );
-    assert (array_group3_concat_unique_weak a1 a3)
+    assert (array_group_concat_unique_weak a1 a3)
 
-let array_group3_one_or_more #b (a: array_group3 b) : array_group3 b =
-  a `array_group3_concat` array_group3_zero_or_more a
+let array_group_one_or_more #b (a: array_group b) : array_group b =
+  a `array_group_concat` array_group_zero_or_more a
 
-let array_group3_one_or_more_equiv #b
- (a1 a2: array_group3 b)
+let array_group_one_or_more_equiv #b
+ (a1 a2: array_group b)
 : Lemma
-  (requires array_group3_equiv a1 a2)
-  (ensures array_group3_equiv (array_group3_one_or_more a1) (array_group3_one_or_more a2))
-  [SMTPat (array_group3_equiv (array_group3_one_or_more a1) (array_group3_one_or_more a2))]
-= array_group3_zero_or_more_equiv a1 a2
+  (requires array_group_equiv a1 a2)
+  (ensures array_group_equiv (array_group_one_or_more a1) (array_group_one_or_more a2))
+  [SMTPat (array_group_equiv (array_group_one_or_more a1) (array_group_one_or_more a2))]
+= array_group_zero_or_more_equiv a1 a2
 
-let array_group3_zero_or_one #b (a: array_group3 b) : Tot (array_group3 b) =
-  a `array_group3_choice` array_group3_empty
+let array_group_zero_or_one #b (a: array_group b) : Tot (array_group b) =
+  a `array_group_choice` array_group_empty
 
-val array_group3_concat_unique_strong_concat_left
+val array_group_concat_unique_strong_concat_left
   (#b: _)
-  (g1 g2 g3: array_group3 b)
+  (g1 g2 g3: array_group b)
 : Lemma
   (requires
-    array_group3_concat_unique_strong g1 (array_group3_concat g2 g3) /\
-    array_group3_concat_unique_strong g2 g3 /\
-    array_group3_concat_unique_weak g1 g2
+    array_group_concat_unique_strong g1 (array_group_concat g2 g3) /\
+    array_group_concat_unique_strong g2 g3 /\
+    array_group_concat_unique_weak g1 g2
   )
   (ensures
-    array_group3_concat_unique_strong (array_group3_concat g1 g2) g3
+    array_group_concat_unique_strong (array_group_concat g1 g2) g3
   )
 
-val array_group3_concat_unique_strong_zero_or_one_left
-  (#b: _) (a1 a2: array_group3 b)
+val array_group_concat_unique_strong_zero_or_one_left
+  (#b: _) (a1 a2: array_group b)
 : Lemma
   (requires (
-    array_group3_disjoint a1 a2 /\
-    array_group3_concat_unique_strong a1 a2
+    array_group_disjoint a1 a2 /\
+    array_group_concat_unique_strong a1 a2
   ))
   (ensures (
-    array_group3_concat_unique_strong (array_group3_zero_or_one a1) a2
+    array_group_concat_unique_strong (array_group_zero_or_one a1) a2
   ))
 
-val array_group3_concat_unique_strong_one_or_more_left
-  (#b: _) (a1 a2: array_group3 b)
+val array_group_concat_unique_strong_one_or_more_left
+  (#b: _) (a1 a2: array_group b)
 : Lemma
   (requires (
-    array_group3_disjoint a1 a2 /\
-    array_group3_concat_unique_strong a1 a1 /\
-    array_group3_concat_unique_strong a1 a2
+    array_group_disjoint a1 a2 /\
+    array_group_concat_unique_strong a1 a1 /\
+    array_group_concat_unique_strong a1 a2
   ))
   (ensures (
-    array_group3_concat_unique_strong (array_group3_one_or_more a1) a2
+    array_group_concat_unique_strong (array_group_one_or_more a1) a2
   ))
 
-val array_group3_concat_unique_weak_zero_or_one_left
-  (#b: _) (a1 a2: array_group3 b)
+val array_group_concat_unique_weak_zero_or_one_left
+  (#b: _) (a1 a2: array_group b)
 : Lemma
   (requires (
-    array_group3_disjoint a1 a2 /\
-    array_group3_concat_unique_weak a1 a2
+    array_group_disjoint a1 a2 /\
+    array_group_concat_unique_weak a1 a2
   ))
   (ensures (
-    array_group3_concat_unique_weak (array_group3_zero_or_one a1) a2
+    array_group_concat_unique_weak (array_group_zero_or_one a1) a2
   ))
 
-val array_group3_concat_unique_weak_one_or_more_left
-  (#b: _) (a1 a2: array_group3 b)
+val array_group_concat_unique_weak_one_or_more_left
+  (#b: _) (a1 a2: array_group b)
 : Lemma
   (requires (
-    array_group3_disjoint a1 a2 /\
-    array_group3_concat_unique_strong a1 a1 /\
-    array_group3_concat_unique_weak a1 a2
+    array_group_disjoint a1 a2 /\
+    array_group_concat_unique_strong a1 a1 /\
+    array_group_concat_unique_weak a1 a2
   ))
   (ensures (
-    array_group3_concat_unique_weak (array_group3_one_or_more a1) a2
+    array_group_concat_unique_weak (array_group_one_or_more a1) a2
   ))
 
-let array_group3_item (#b: option Cbor.cbor) (t: bounded_typ_gen b) : array_group3 b = fun l ->
+let array_group_item (#b: option Cbor.cbor) (t: bounded_typ_gen b) : array_group b = fun l ->
   match l with
   | [] -> None
   | a :: q -> if t a then Some ([a], q) else None
 
-let array_group3_item_equiv
+let array_group_item_equiv
   #b
   (t1 t2: bounded_typ_gen b)
 : Lemma
   (requires (t1 `typ_equiv` t2))
-  (ensures (array_group3_item t1 `array_group3_equiv` array_group3_item t2))
+  (ensures (array_group_item t1 `array_group_equiv` array_group_item t2))
 = ()
 
-let match_array_group3 (#b: option Cbor.cbor) (a: array_group3 b)
+let match_array_group (#b: option Cbor.cbor) (a: array_group b)
   (l: list Cbor.cbor {opt_precedes_list l b})
 : Tot bool
 = match a l with
   | Some (_, l') -> Nil? l'
   | _ -> false
 
-let t_array3 (#b: option Cbor.cbor) (a: array_group3 b) : bounded_typ_gen b = fun w -> let x = Cbor.unpack w in
+let t_array3 (#b: option Cbor.cbor) (a: array_group b) : bounded_typ_gen b = fun w -> let x = Cbor.unpack w in
   Cbor.CArray? x &&
-  match_array_group3 a (Cbor.CArray?.v x)
+  match_array_group a (Cbor.CArray?.v x)
 
 let t_array3_equiv
   #b
-  (a1 a2: array_group3 b)
+  (a1 a2: array_group b)
 : Lemma
-  (requires (array_group3_equiv a1 a2))
+  (requires (array_group_equiv a1 a2))
   (ensures (typ_equiv (t_array3 a1) (t_array3 a2)))
 = ()
 
 let close_array_group
   (#b: _)
-  (t: array_group3 b)
-: Tot (array_group3 b)
+  (t: array_group b)
+: Tot (array_group b)
 = fun l ->
     let res = t l in
     match res with
@@ -508,16 +524,16 @@ let close_array_group
 
 let maybe_close_array_group
   (#b: _)
-  (t: array_group3 b)
+  (t: array_group b)
   (close: bool)
-: Tot (array_group3 b)
+: Tot (array_group b)
 = if close
   then close_array_group t
   else t
 
 let array3_close_array_group
   (#b: _)
-  (a: array_group3 b)
+  (a: array_group b)
 : Lemma
   (typ_equiv
     (t_array3 a)
@@ -535,16 +551,16 @@ let array3_close_array_group
 // to the "size" annotation in a sized type.)
 
 let rec t_array3_rec
-  (phi: (b: Cbor.cbor) -> (bounded_typ b -> array_group3 (Some b)))
+  (phi: (b: Cbor.cbor) -> (bounded_typ b -> array_group (Some b)))
   (w: Cbor.cbor)
 : Tot bool
   (decreases w)
 = let x = Cbor.unpack w in
   Cbor.CArray? x &&
-  match_array_group3 (phi w (t_array3_rec phi)) (Cbor.CArray?.v x)
+  match_array_group (phi w (t_array3_rec phi)) (Cbor.CArray?.v x)
 
 let array_group_parser_spec_arg
-  (source: array_group3 None)
+  (source: array_group None)
 : Tot Type0
 = (x: list Cbor.cbor {
    match source x with
@@ -553,7 +569,7 @@ let array_group_parser_spec_arg
   })
 
 let array_group_parser_spec_ret
-  (source: array_group3 None)
+  (source: array_group None)
   (#target: Type0)
   (target_size: target -> Tot nat)
   (target_prop: target -> prop)
@@ -565,7 +581,7 @@ let array_group_parser_spec_ret
   })
 
 let array_group_parser_spec
-  (source: array_group3 None)
+  (source: array_group None)
   (#target: Type0)
   (target_size: target -> Tot nat)
   (target_prop: target -> prop)
@@ -573,7 +589,7 @@ let array_group_parser_spec
 = (x: array_group_parser_spec_arg source) -> Tot (array_group_parser_spec_ret source target_size target_prop x)
 
 let array_group_serializer_spec
-  (#source: array_group3 None)
+  (#source: array_group None)
   (#target: Type0)
   (#target_size: target -> Tot nat)
   (#target_prop: target -> prop)
@@ -585,7 +601,7 @@ let array_group_serializer_spec
 
 noeq
 type ag_spec
-  (source: array_group3 None)
+  (source: array_group None)
   (target: Type0)
 = {
   ag_size: target -> Tot nat;
@@ -595,7 +611,7 @@ type ag_spec
 }
 
 let ag_spec_coerce_target_prop
-  (#source: array_group3 None)
+  (#source: array_group None)
   (#target: Type0)
   (p: ag_spec source target)
   (target_size': target -> Tot nat {
@@ -613,7 +629,7 @@ let ag_spec_coerce_target_prop
 }
 
 let parser_spec_array_group
-  (#source: array_group3 None)
+  (#source: array_group None)
   (#target: Type0)
   (#target_size: target -> Tot nat)
   (#target_prop: target -> prop)
@@ -625,7 +641,7 @@ let parser_spec_array_group
 = fun x -> let Cbor.CArray a = Cbor.unpack x in p a
 
 let serializer_spec_array_group
-  (#source: array_group3 None)
+  (#source: array_group None)
   (#target: Type0)
   (#target_size: target -> Tot nat)
   (#target_prop: target -> prop)
@@ -638,7 +654,7 @@ let serializer_spec_array_group
 = fun x -> Cbor.pack (Cbor.CArray (s x))
 
 let spec_array_group_serializable
-  (#source: array_group3 None)
+  (#source: array_group None)
   (#target: Type0)
   (p: ag_spec source target)
   (x: target)
@@ -647,7 +663,7 @@ let spec_array_group_serializable
   p.ag_size x < pow2 64
 
 let spec_array_group
-  (#source: array_group3 None)
+  (#source: array_group None)
   (#target: Type0)
   (p: ag_spec source target)
 : Tot (spec (t_array3 source) target)
@@ -658,7 +674,7 @@ let spec_array_group
 }
 
 let array_group_parser_spec_bij
-  (#source: array_group3 None)
+  (#source: array_group None)
   (#target1: Type0)
   (#target_size1: target1 -> Tot nat)
   (#target_prop1: target1 -> prop)
@@ -674,7 +690,7 @@ let array_group_parser_spec_bij
 = fun x -> bij.bij_from_to (f x)
 
 let array_group_serializer_spec_bij
-  (#source: array_group3 None)
+  (#source: array_group None)
   (#target1: Type0)
   (#target_size1: target1 -> Tot nat)
   (#target_prop1: target1 -> prop)
@@ -691,7 +707,7 @@ let array_group_serializer_spec_bij
 = fun x -> s (bij.bij_to_from x)
 
 let ag_spec_bij_size
-  (#source: array_group3 None)
+  (#source: array_group None)
   (#target1: Type0)
   (f: ag_spec source target1)
   (#target2: Type0)
@@ -701,7 +717,7 @@ let ag_spec_bij_size
 = f.ag_size (bij.bij_to_from x2)
 
 let ag_spec_bij_serializable
-  (#source: array_group3 None)
+  (#source: array_group None)
   (#target1: Type0)
   (f: ag_spec source target1)
   (#target2: Type0)
@@ -711,7 +727,7 @@ let ag_spec_bij_serializable
 = f.ag_serializable (bij.bij_to_from x2)
 
 let ag_spec_bij
-  (#source: array_group3 None)
+  (#source: array_group None)
   (#target1: Type0)
   (f: ag_spec source target1)
   (#target2: Type0)
@@ -732,10 +748,10 @@ let array_group_parser_spec_item
   (target_size: target -> Tot nat {
     forall x . target_size x == 1
   })
-: Tot (array_group_parser_spec (array_group3_item ty) target_size target_prop)
+: Tot (array_group_parser_spec (array_group_item ty) target_size target_prop)
 = fun x -> let [hd] = x in p hd
 
-let array_group_serializer_spec_item
+val array_group_serializer_spec_item
   (#ty: typ)
   (#target: Type)
   (#target_prop: target -> GTot prop)
@@ -745,7 +761,20 @@ let array_group_serializer_spec_item
     forall x . target_size x == 1
   })
 : Tot (array_group_serializer_spec (array_group_parser_spec_item p target_size))
-= fun x -> [s x]
+
+val array_group_serializer_spec_item_eq
+  (#ty: typ)
+  (#target: Type)
+  (#target_prop: target -> GTot prop)
+  (#p: parser_spec ty target target_prop)
+  (s: serializer_spec p)
+  (target_size: target -> Tot nat {
+    forall x . target_size x == 1
+  })
+  (x: target { target_prop x })
+: Lemma
+  (ensures (array_group_serializer_spec_item s target_size x == [s x]))
+  [SMTPat (array_group_serializer_spec_item s target_size x)]
 
 let ag_spec_item_size
   (target: Type)
@@ -757,7 +786,7 @@ let ag_spec_item
   (#ty: typ)
   (#target: Type)
   (p: spec ty target)
-: Tot (ag_spec (array_group3_item ty) target)
+: Tot (ag_spec (array_group_item ty) target)
 = {
   ag_size = ag_spec_item_size target;
   ag_serializable = p.serializable;
@@ -766,17 +795,17 @@ let ag_spec_item
 }
 
 val array_group_parser_spec_concat
-  (#source1: array_group3 None)
+  (#source1: array_group None)
   (#target1: Type)
   (#target_size1: target1 -> Tot nat)
   (#target_prop1: target1 -> prop)
   (p1: array_group_parser_spec source1 target_size1 target_prop1)
-  (#source2: array_group3 None)
+  (#source2: array_group None)
   (#target2: Type)
   (#target_size2: target2 -> Tot nat)
   (#target_prop2: target2 -> prop)
   (p2: array_group_parser_spec source2 target_size2 target_prop2 {
-    array_group3_concat_unique_weak source1 source2
+    array_group_concat_unique_weak source1 source2
   })
   (target_size: (target1 & target2) -> Tot nat {
     forall x . target_size x == target_size1 (fst x) + target_size2 (snd x)
@@ -784,22 +813,22 @@ val array_group_parser_spec_concat
   (target_prop: (target1 & target2) -> prop {
     forall x . target_prop x <==> (target_prop1 (fst x) /\ target_prop2 (snd x))
   })
-: Tot (array_group_parser_spec (array_group3_concat source1 source2) target_size target_prop)
+: Tot (array_group_parser_spec (array_group_concat source1 source2) target_size target_prop)
 
 #restart-solver
 
 val array_group_parser_spec_concat_eq
-  (#source1: array_group3 None)
+  (#source1: array_group None)
   (#target1: Type)
   (#target_size1: target1 -> Tot nat)
   (#target_prop1: target1 -> prop)
   (p1: array_group_parser_spec source1 target_size1 target_prop1)
-  (#source2: array_group3 None)
+  (#source2: array_group None)
   (#target2: Type)
   (#target_size2: target2 -> Tot nat)
   (#target_prop2: target2 -> prop)
   (p2: array_group_parser_spec source2 target_size2 target_prop2 {
-    array_group3_concat_unique_weak source1 source2
+    array_group_concat_unique_weak source1 source2
   })
   (target_size: (target1 & target2) -> Tot nat {
     forall x . target_size x == target_size1 (fst x) + target_size2 (snd x)
@@ -807,7 +836,7 @@ val array_group_parser_spec_concat_eq
   (target_prop: (target1 & target2) -> prop {
     forall x . target_prop x <==> (target_prop1 (fst x) /\ target_prop2 (snd x))
   })
-  (x: array_group_parser_spec_arg (array_group3_concat source1 source2))
+  (x: array_group_parser_spec_arg (array_group_concat source1 source2))
 : Lemma
   (let Some (x1, x2) = source1 x in
     source1 x1 == Some (x1, []) /\
@@ -817,19 +846,19 @@ val array_group_parser_spec_concat_eq
   [SMTPat (array_group_parser_spec_concat p1 p2 target_size target_prop x)]
 
 let array_group_serializer_spec_concat
-  (#source1: array_group3 None)
+  (#source1: array_group None)
   (#target1: Type)
   (#target_size1: target1 -> Tot nat)
   (#target_prop1: target1 -> prop)
   (#p1: array_group_parser_spec source1 target_size1 target_prop1)
   (s1: array_group_serializer_spec p1)
-  (#source2: array_group3 None)
+  (#source2: array_group None)
   (#target2: Type)
   (#target_size2: target2 -> Tot nat)
   (#target_prop2: target2 -> prop)
   (#p2: array_group_parser_spec source2 target_size2 target_prop2)
   (s2: array_group_serializer_spec p2 {
-    array_group3_concat_unique_weak source1 source2
+    array_group_concat_unique_weak source1 source2
   })
   (target_size: (target1 & target2) -> Tot nat {
     forall x . target_size x == target_size1 (fst x) + target_size2 (snd x)
@@ -843,14 +872,14 @@ let array_group_serializer_spec_concat
     let l1 = s1 x1 in
     let l2 = s2 x2 in
     let res = l1 `List.Tot.append` l2 in
-    array_group3_concat_unique_weak_elim2 source1 source2 l1 l2;
+    array_group_concat_unique_weak_elim2 source1 source2 l1 l2;
     res
 
 let ag_spec_concat_size
-  (#source1: array_group3 None)
+  (#source1: array_group None)
   (#target1: Type)
   (p1: ag_spec source1 target1)
-  (#source2: array_group3 None)
+  (#source2: array_group None)
   (#target2: Type)
   (p2: ag_spec source2 target2)
   (x: (target1 & target2))
@@ -858,10 +887,10 @@ let ag_spec_concat_size
 = p1.ag_size (fst x) + p2.ag_size (snd x)
 
 let ag_spec_concat_serializable
-  (#source1: array_group3 None)
+  (#source1: array_group None)
   (#target1: Type)
   (p1: ag_spec source1 target1)
-  (#source2: array_group3 None)
+  (#source2: array_group None)
   (#target2: Type)
   (p2: ag_spec source2 target2)
   (x: (target1 & target2))
@@ -869,15 +898,15 @@ let ag_spec_concat_serializable
 = p1.ag_serializable (fst x) /\ p2.ag_serializable (snd x)
 
 let ag_spec_concat
-  (#source1: array_group3 None)
+  (#source1: array_group None)
   (#target1: Type)
   (p1: ag_spec source1 target1)
-  (#source2: array_group3 None)
+  (#source2: array_group None)
   (#target2: Type)
   (p2: ag_spec source2 target2 {
-    array_group3_concat_unique_weak source1 source2
+    array_group_concat_unique_weak source1 source2
   })
-: Tot (ag_spec (array_group3_concat source1 source2) (target1 & target2))
+: Tot (ag_spec (array_group_concat source1 source2) (target1 & target2))
 = {
   ag_size = ag_spec_concat_size p1 p2;
   ag_serializable = ag_spec_concat_serializable p1 p2;
@@ -886,12 +915,12 @@ let ag_spec_concat
 }
 
 let rec array_group_parser_spec_zero_or_more'
-  (#source: array_group3 None)
+  (#source: array_group None)
   (#target: Type)
   (#target_size: target -> Tot nat)
   (#target_prop: target -> prop)
   (p: array_group_parser_spec source target_size target_prop {
-    array_group3_concat_unique_strong source source
+    array_group_concat_unique_strong source source
   })
   (target_size' : list target -> Tot nat {
     forall (l: list target) . target_size' l == (if Nil? l then 0 else target_size (List.Tot.hd l) + target_size' (List.Tot.tl l))
@@ -899,8 +928,8 @@ let rec array_group_parser_spec_zero_or_more'
   (target_prop' : list target -> prop {
     forall x . target_prop' x <==> (forall y . List.Tot.memP y x ==> target_prop y)
   })
-  (x: array_group_parser_spec_arg (array_group3_zero_or_more source))
-: Tot (array_group_parser_spec_ret (array_group3_zero_or_more source) target_size' target_prop' x)
+  (x: array_group_parser_spec_arg (array_group_zero_or_more source))
+: Tot (array_group_parser_spec_ret (array_group_zero_or_more source) target_size' target_prop' x)
   (decreases (List.Tot.length x))
 = match source x with
   | None ->
@@ -913,19 +942,19 @@ let rec array_group_parser_spec_zero_or_more'
     if Nil? l1
     then []
     else begin
-      array_group3_concat_unique_weak_zero_or_more_right source source;
+      array_group_concat_unique_weak_zero_or_more_right source source;
       List.Tot.append_length l1 l2;
       let q = array_group_parser_spec_zero_or_more' p target_size' target_prop' l2 in
       p l1 :: q
     end
 
 let array_group_parser_spec_zero_or_more
-  (#source: array_group3 None)
+  (#source: array_group None)
   (#target: Type)
   (#target_size: target -> Tot nat)
   (#target_prop: target -> prop)
   (p: array_group_parser_spec source target_size target_prop {
-    array_group3_concat_unique_strong source source
+    array_group_concat_unique_strong source source
   })
   (target_size' : list target -> Tot nat {
     forall (l: list target) . target_size' l == (if Nil? l then 0 else target_size (List.Tot.hd l) + target_size' (List.Tot.tl l))
@@ -933,25 +962,25 @@ let array_group_parser_spec_zero_or_more
   (target_prop' : list target -> prop {
     forall x . target_prop' x <==> (forall y . List.Tot.memP y x ==> target_prop y)
   })
-: Tot (array_group_parser_spec (array_group3_zero_or_more source) target_size' target_prop')
+: Tot (array_group_parser_spec (array_group_zero_or_more source) target_size' target_prop')
 = array_group_parser_spec_zero_or_more' p target_size' target_prop'
 
-let array_group3_is_nonempty (a: array_group3 None) : Tot prop =
+let array_group_is_nonempty (a: array_group None) : Tot prop =
     forall l . match a l with
     | Some (consumed, _) -> Cons? consumed
     | _ -> True
 
-let nonempty_array_group3 : Type0 =
-  (a: array_group3 None { array_group3_is_nonempty a })
+let nonempty_array_group : Type0 =
+  (a: array_group None { array_group_is_nonempty a })
 
 let rec array_group_serializer_spec_zero_or_more'
-  (#source: nonempty_array_group3)
+  (#source: nonempty_array_group)
   (#target: Type)
   (#target_size: target -> Tot nat)
   (#target_prop: target -> prop)
   (#p: array_group_parser_spec source target_size target_prop)
   (s: array_group_serializer_spec p {
-    array_group3_concat_unique_strong source source
+    array_group_concat_unique_strong source source
   })
   (target_size' : list target -> Tot nat {
     forall (l: list target) . target_size' l == (if Nil? l then 0 else target_size (List.Tot.hd l) + target_size' (List.Tot.tl l))
@@ -960,27 +989,27 @@ let rec array_group_serializer_spec_zero_or_more'
     forall x . target_prop' x <==> (forall y . List.Tot.memP y x ==> target_prop y)
   })
   (x: list target { target_prop' x })
-: Tot (y: array_group_parser_spec_arg (array_group3_zero_or_more source) {
+: Tot (y: array_group_parser_spec_arg (array_group_zero_or_more source) {
     array_group_parser_spec_zero_or_more p target_size' target_prop' y == x
   })
   (decreases x)
 = match x with
   | [] -> []
   | a :: q ->
-    array_group3_concat_unique_weak_zero_or_more_right source source;
+    array_group_concat_unique_weak_zero_or_more_right source source;
     let l1 = s a in
     let l2 = array_group_serializer_spec_zero_or_more' s target_size' target_prop' q in
     let res = l1 `List.Tot.append` l2 in
     res
 
 let array_group_serializer_spec_zero_or_more
-  (#source: nonempty_array_group3)
+  (#source: nonempty_array_group)
   (#target: Type)
   (#target_size: target -> Tot nat)
   (#target_prop: target -> prop)
   (#p: array_group_parser_spec source target_size target_prop)
   (s: array_group_serializer_spec p {
-    array_group3_concat_unique_strong source source
+    array_group_concat_unique_strong source source
   })
   (target_size' : list target -> Tot nat {
     forall (l: list target) . target_size' l == (if Nil? l then 0 else target_size (List.Tot.hd l) + target_size' (List.Tot.tl l))
@@ -992,7 +1021,7 @@ let array_group_serializer_spec_zero_or_more
 = array_group_serializer_spec_zero_or_more' s target_size' target_prop'
 
 let rec ag_spec_zero_or_more_size
-  (#source: array_group3 None)
+  (#source: array_group None)
   (#target: Type)
   (p: ag_spec source target)
   (l: list target)
@@ -1003,7 +1032,7 @@ let rec ag_spec_zero_or_more_size
   | hd :: tl -> p.ag_size hd + ag_spec_zero_or_more_size p tl
 
 let ag_spec_zero_or_more_serializable
-  (#source: array_group3 None)
+  (#source: array_group None)
   (#target: Type)
   (p: ag_spec source target)
   (x: list target)
@@ -1011,12 +1040,12 @@ let ag_spec_zero_or_more_serializable
 = forall y . List.Tot.memP y x ==> p.ag_serializable y
 
 let ag_spec_zero_or_more
-  (#source: nonempty_array_group3)
+  (#source: nonempty_array_group)
   (#target: Type)
   (p: ag_spec source target {
-    array_group3_concat_unique_strong source source
+    array_group_concat_unique_strong source source
   })
-: Tot (ag_spec (array_group3_zero_or_more source) (list target))
+: Tot (ag_spec (array_group_zero_or_more source) (list target))
 = {
   ag_size = ag_spec_zero_or_more_size p;
   ag_serializable = ag_spec_zero_or_more_serializable p;
@@ -1025,12 +1054,12 @@ let ag_spec_zero_or_more
 }
 
 let array_group_parser_spec_one_or_more
-  (#source: array_group3 None)
+  (#source: array_group None)
   (#target: Type)
   (#target_size: target -> Tot nat)
   (#target_prop: target -> prop)
   (p: array_group_parser_spec source target_size target_prop {
-    array_group3_concat_unique_strong source source
+    array_group_concat_unique_strong source source
   })
   (target_size1 : list target -> Tot nat {
     forall (l: list target) . target_size1 l == (if Nil? l then 0 else target_size (List.Tot.hd l) + target_size1 (List.Tot.tl l))
@@ -1038,21 +1067,21 @@ let array_group_parser_spec_one_or_more
   (target_prop1 : list target -> prop {
     forall x . target_prop1 x <==> (Cons? x /\ (forall y . List.Tot.memP y x ==> target_prop y))
   })
-: Tot (array_group_parser_spec (array_group3_one_or_more source) target_size1 target_prop1)
+: Tot (array_group_parser_spec (array_group_one_or_more source) target_size1 target_prop1)
 = fun x ->
-  array_group3_concat_unique_weak_zero_or_more_right source source;
+  array_group_concat_unique_weak_zero_or_more_right source source;
   let Some (l1, l2) = source x in
   List.Tot.append_length l1 l2;
   p l1 :: array_group_parser_spec_zero_or_more p target_size1 (fun x -> Nil? x \/ target_prop1 x) l2
 
 let array_group_serializer_spec_one_or_more
-  (#source: nonempty_array_group3)
+  (#source: nonempty_array_group)
   (#target: Type)
   (#target_size: target -> Tot nat)
   (#target_prop: target -> prop)
   (#p: array_group_parser_spec source target_size target_prop)
   (s: array_group_serializer_spec p {
-    array_group3_concat_unique_strong source source
+    array_group_concat_unique_strong source source
   })
   (target_size1 : list target -> Tot nat {
     forall (l: list target) . target_size1 l == (if Nil? l then 0 else target_size (List.Tot.hd l) + target_size1 (List.Tot.tl l))
@@ -1062,7 +1091,7 @@ let array_group_serializer_spec_one_or_more
   })
 : Tot (array_group_serializer_spec (array_group_parser_spec_one_or_more p target_size1 target_prop1))
 = fun x ->
-  array_group3_concat_unique_weak_zero_or_more_right source source;
+  array_group_concat_unique_weak_zero_or_more_right source source;
   let hd :: tl = x in
   let l1 = s hd in
   let l2 = array_group_serializer_spec_zero_or_more s target_size1 (fun x -> Nil? x \/ target_prop1 x) tl in
@@ -1070,7 +1099,7 @@ let array_group_serializer_spec_one_or_more
   l1 `List.Tot.append` l2
 
 let ag_spec_one_or_more_serializable
-  (#source: array_group3 None)
+  (#source: array_group None)
   (#target: Type)
   (p: ag_spec source target)
   (x: list target)
@@ -1079,12 +1108,12 @@ let ag_spec_one_or_more_serializable
   ag_spec_zero_or_more_serializable p x
 
 let ag_spec_one_or_more
-  (#source: nonempty_array_group3)
+  (#source: nonempty_array_group)
   (#target: Type)
   (p: ag_spec source target {
-    array_group3_concat_unique_strong source source
+    array_group_concat_unique_strong source source
   })
-: Tot (ag_spec (array_group3_one_or_more source) (list target))
+: Tot (ag_spec (array_group_one_or_more source) (list target))
 = {
   ag_size = ag_spec_zero_or_more_size p;
   ag_serializable = ag_spec_one_or_more_serializable p;
@@ -1093,12 +1122,12 @@ let ag_spec_one_or_more
 }
 
 let array_group_parser_spec_choice
-  (#source1: array_group3 None)
+  (#source1: array_group None)
   (#target1: Type0)
   (#target_size1: target1 -> Tot nat)
   (#target_prop1: target1 -> prop)
   (p1: array_group_parser_spec source1 target_size1 target_prop1)
-  (#source2: array_group3 None)
+  (#source2: array_group None)
   (#target2: Type0)
   (#target_size2: target2 -> Tot nat)
   (#target_prop2: target2 -> prop)
@@ -1115,25 +1144,25 @@ let array_group_parser_spec_choice
     | Inr x2 -> target_prop2 x2
     end
   })
-: Tot (array_group_parser_spec (source1 `array_group3_choice` source2) target_size target_prop)
+: Tot (array_group_parser_spec (source1 `array_group_choice` source2) target_size target_prop)
 = fun x ->
     if Some? (source1 x)
     then Inl (p1 x)
     else Inr (p2 x)
 
 let array_group_serializer_spec_choice
-  (#source1: array_group3 None)
+  (#source1: array_group None)
   (#target1: Type0)
   (#target_size1: target1 -> Tot nat)
   (#target_prop1: target1 -> prop)
   (#p1: array_group_parser_spec source1 target_size1 target_prop1)
   (s1: array_group_serializer_spec p1)
-  (#source2: array_group3 None)
+  (#source2: array_group None)
   (#target2: Type0)
   (#target_size2: target2 -> Tot nat)
   (#target_prop2: target2 -> prop)
   (#p2: array_group_parser_spec source2 target_size2 target_prop2)
-  (s2: array_group_serializer_spec p2 { source1 `array_group3_disjoint` source2 }) // disjointness needed to avoid the CBOR object serialized from one case to be parsed into the other case
+  (s2: array_group_serializer_spec p2 { source1 `array_group_disjoint` source2 }) // disjointness needed to avoid the CBOR object serialized from one case to be parsed into the other case
   (target_size: (target1 `either` target2) -> Tot nat {
     forall x . target_size x == begin match x with
     | Inl y -> target_size1 y
@@ -1152,10 +1181,10 @@ let array_group_serializer_spec_choice
   | Inr y -> s2 y
 
 let ag_spec_choice_size
-  (#source1: array_group3 None)
+  (#source1: array_group None)
   (#target1: Type0)
   (p1: ag_spec source1 target1)
-  (#source2: array_group3 None)
+  (#source2: array_group None)
   (#target2: Type0)
   (p2: ag_spec source2 target2)
   (x: either target1 target2)
@@ -1165,10 +1194,10 @@ let ag_spec_choice_size
   | Inr x2 -> p2.ag_size x2
 
 let ag_spec_choice_serializable
-  (#source1: array_group3 None)
+  (#source1: array_group None)
   (#target1: Type0)
   (p1: ag_spec source1 target1)
-  (#source2: array_group3 None)
+  (#source2: array_group None)
   (#target2: Type0)
   (p2: ag_spec source2 target2)
   (x: either target1 target2)
@@ -1178,13 +1207,13 @@ let ag_spec_choice_serializable
   | Inr x2 -> p2.ag_serializable x2
 
 let ag_spec_choice
-  (#source1: array_group3 None)
+  (#source1: array_group None)
   (#target1: Type0)
   (p1: ag_spec source1 target1)
-  (#source2: array_group3 None)
+  (#source2: array_group None)
   (#target2: Type0)
-  (p2: ag_spec source2 target2  { source1 `array_group3_disjoint` source2 })
-: Tot (ag_spec (source1 `array_group3_choice` source2) (either target1 target2))
+  (p2: ag_spec source2 target2  { source1 `array_group_disjoint` source2 })
+: Tot (ag_spec (source1 `array_group_choice` source2) (either target1 target2))
 = {
   ag_size = ag_spec_choice_size p1 p2;
   ag_serializable = ag_spec_choice_serializable p1 p2;
@@ -1193,7 +1222,7 @@ let ag_spec_choice
 }
 
 let array_group_parser_spec_zero_or_one
-  (#source: array_group3 None)
+  (#source: array_group None)
   (#target: Type)
   (#target_size: target -> Tot nat)
   (#target_prop: target -> prop)
@@ -1210,14 +1239,14 @@ let array_group_parser_spec_zero_or_one
     | Some x -> target_prop x
     end
   })
-: Tot (array_group_parser_spec (array_group3_zero_or_one source) target_size' target_prop')
+: Tot (array_group_parser_spec (array_group_zero_or_one source) target_size' target_prop')
 = fun x ->
     if Some? (source x)
     then Some (p x)
     else None
 
 let array_group_serializer_spec_zero_or_one
-  (#source: nonempty_array_group3) // needed because the empty case must map to None only
+  (#source: nonempty_array_group) // needed because the empty case must map to None only
   (#target: Type)
   (#target_size: target -> Tot nat)
   (#target_prop: target -> prop)
@@ -1242,7 +1271,7 @@ let array_group_serializer_spec_zero_or_one
     | Some y -> s y
 
 let ag_spec_zero_or_one_size
-  (#source: nonempty_array_group3)
+  (#source: nonempty_array_group)
   (#target: Type)
   (p: ag_spec source target)
   (x: option target)
@@ -1252,7 +1281,7 @@ let ag_spec_zero_or_one_size
   | Some x' -> p.ag_size x'
 
 let ag_spec_zero_or_one_serializable
-  (#source: nonempty_array_group3)
+  (#source: nonempty_array_group)
   (#target: Type)
   (p: ag_spec source target)
   (x: option target)
@@ -1262,10 +1291,10 @@ let ag_spec_zero_or_one_serializable
   | Some x' -> p.ag_serializable x'
 
 let ag_spec_zero_or_one
-  (#source: nonempty_array_group3)
+  (#source: nonempty_array_group)
   (#target: Type)
   (p: ag_spec source target)
-: Tot (ag_spec (array_group3_zero_or_one source) (option target))
+: Tot (ag_spec (array_group_zero_or_one source) (option target))
 = {
   ag_size = ag_spec_zero_or_one_size p;
   ag_serializable = ag_spec_zero_or_one_serializable p;
